

$\chi(\sum_i k_i = k) = 0$  otherwise. The matrices  $E_{ij}^{(k)}$  are defined for  $k = 0, 1, 2$  as

$$E_{ij}^{(0)} = D_{ij} = \bar{\alpha}_i \delta_{ij}, \quad E_{ij}^{(1)} = \bar{B}_{ij}(\varepsilon), \quad E_{ij}^{(2)} = \delta_{ij}, \quad (\text{S15})$$

corresponding to the matrices  $\mathbf{D}$ ,  $\bar{\mathbf{B}}$ , and  $\mathbf{I}$  in Eq. (S11), respectively ( $\delta_{ij}$  is the Kronecker delta function). Equations (S14) and (S15) provide an expression for the coefficients of  $\det(\bar{\mathbf{J}} - \nu \mathbf{I})$  in terms of  $\beta$ , and thus of  $\varepsilon$ , for a given system and its matrix  $\mathbf{P}$ .

We now derive a different expression for  $\det(\bar{\mathbf{J}} - \nu \mathbf{I})$ , this time in terms of the characteristic polynomial coefficients  $c_i$  and  $d_i$ , using Eq. (S9). Ignoring the dependence of  $c_i$  and  $d_i$  on  $\varepsilon$  for the moment and regarding them as independent variables, the coefficient of the  $\nu^k$  term can be written as

$$\sum_{\{k_i\}} \prod_{i=1}^n a_i^{(k_i)} \cdot \chi(\sum_i k_i = k), \quad (\text{S16})$$

where the summation is the same as in Eq. (S14) and

$$a_i^{(0)} = d_i, \quad a_i^{(1)} = c_i, \quad a_i^{(2)} = 1. \quad (\text{S17})$$

Setting Eqs. (S14) and (S16) equal to each other, we obtain a set of nonlinear equations that must be satisfied by the variables  $c_1, \dots, c_n, d_1, \dots, d_n$ , and  $\varepsilon$ :

$$F_k(c_1, \dots, c_n, d_1, \dots, d_n, \varepsilon) = 0, \quad k = 1, 2, \dots, 2n-1, \quad (\text{S18})$$

or, in vector form,

$$\mathbf{F}(c_1, \dots, c_n, d_1, \dots, d_n, \varepsilon) = \mathbf{0}, \quad (\text{S19})$$

where we have defined  $\mathbf{F} \equiv (F_1, \dots, F_{2n-1})^T$ , and the functions  $F_k$  are given by

$$\begin{aligned} F_k &= \sum_{\{k_i\}} \prod_{i=1}^n a_i^{(k_i)} \cdot \chi(\sum_i k_i = k) - \sum_{\sigma} \text{sign}(\sigma) \sum_{\{k_i\}} \prod_{i=1}^n E_{i\sigma(i)}^{(k_i)} \cdot \chi(\sum_i k_i = k) \\ &= \sum_{\{k_i\}} \chi(\sum_i k_i = k) \cdot \left[ \prod_{i=1}^n a_i^{(k_i)} - \sum_{\sigma} \text{sign}(\sigma) \prod_{i=1}^n E_{i\sigma(i)}^{(k_i)} \right]. \end{aligned} \quad (\text{S20})$$

This is the equation that implicitly defines the functions  $c_i = c_i(\varepsilon)$  and  $d_i = d_i(\varepsilon)$ . Note that, when  $c_i = 1$ ,  $d_i = \bar{\alpha}_i$ , and  $\varepsilon = 0$  (corresponding to the point  $\beta_{=}$ ), we have  $E_{ij}^{(1)} = \bar{B}_{ij}(0) = \delta_{ij}$ , and hence

$$a_i^{(0)} = d_i(0) = \bar{\alpha}_i, \quad a_i^{(1)} = c_i(0) = 1, \quad a_i^{(2)} = 1, \quad E_{ij}^{(k)} = a_i^{(k)} \delta_{ij}, \quad (\text{S21})$$

implying

$$\begin{aligned} F_k(1, \dots, 1, \bar{\alpha}_1, \dots, \bar{\alpha}_n, 0) &= \sum_{\{k_i\}} \chi(\sum_i k_i = k) \cdot \left[ \prod_{i=1}^n a_i^{(k_i)} - \sum_{\sigma} \text{sign}(\sigma) \prod_{i=1}^n a_{i\sigma(i)}^{(k_i)} \delta_{i\sigma(i)} \right] \\ &= \sum_{\{k_i\}} \chi(\sum_i k_i = k) \cdot \left[ \prod_{i=1}^n a_i^{(k_i)} - \prod_{i=1}^n a_i^{(k_i)} \right] = 0, \end{aligned}$$

i.e., Eq. (S18) is satisfied. The functions  $c_i(\varepsilon)$  and  $d_i(\varepsilon)$  defined through Eq. (S20) thus satisfy  $c_i(0) = 1$  and  $d_i(0) = \bar{\alpha}_i$ .

### 3 Characterizing descending paths on $\lambda^{\max}$ -landscape

Here, we will apply the IFT to show that the functions  $c_i(\varepsilon)$  and  $d_i(\varepsilon)$  are continuously differentiable for small  $\varepsilon$  (and thus define a smooth curve in the neighborhood of the point  $(1, \bar{\alpha}_i)$  in the  $(c_i, d_i)$ -plane), and we determine their first derivatives. The condition under which we can apply the IFT to Eq. (S18) at the point  $(c_1, \dots, c_n, d_1, \dots, d_n, \varepsilon) = (1, \dots, 1, \bar{\alpha}_1, \dots, \bar{\alpha}_n, 0)$  is that the  $(2n - 1) \times (2n - 1)$  matrix

$$\mathbf{G} \equiv \begin{pmatrix} \frac{\partial F_1}{\partial c_1} & \dots & \frac{\partial F_1}{\partial c_n} & \frac{\partial F_1}{\partial d_2} & \dots & \frac{\partial F_1}{\partial d_n} \\ \vdots & & \vdots & \vdots & & \vdots \\ \frac{\partial F_{2n-1}}{\partial c_1} & \dots & \frac{\partial F_{2n-1}}{\partial c_n} & \frac{\partial F_{2n-1}}{\partial d_2} & \dots & \frac{\partial F_{2n-1}}{\partial d_n} \end{pmatrix}, \quad (\text{S22})$$

is non-singular, where the elements of  $\mathbf{G}$  are all evaluated at that point. We note that  $d_1$  is excluded from the set of variables here because  $d_1 = 0$  always holds. We also note that  $\mathbf{G}$  (and whether it is singular or not) is completely determined by  $\bar{\alpha}_2, \dots, \bar{\alpha}_n$ , and hence by the matrix  $\mathbf{P}$  (see examples in Sec. 4). For notational convenience, define  $x_s = c_s$  for  $s = 1, \dots, n$  and  $x_s = d_{s-n+1}$  for  $s = n + 1, \dots, 2n - 1$ . Differentiating Eq. (S20), we find an expression for the  $(k, s)$ -element of  $\mathbf{G}$ :

$$G_{ks} = \frac{\partial F_k}{\partial x_s}(1, \dots, 1, \bar{\alpha}_1, \dots, \bar{\alpha}_n, 0) = \begin{cases} \sum_{\{k_i\}} \prod_{i \neq s} a_i^{(k_i)} \cdot \chi(s, k, \{k_i\}), & \text{if } s = 1, \dots, n, \\ \sum_{\{k_i\}} \prod_{i \neq \hat{s}} a_i^{(k_i)} \cdot \chi(s, k, \{k_i\}), & \text{if } s = n + 1, \dots, 2n - 1, \end{cases} \quad (\text{S23})$$

where the summation is defined as in Eq. (S14); we denote  $\hat{s} \equiv s - n + 1$ ; the values of  $a_i^{(k_i)}$  are given by Eq. (S21); and we have defined

$$\chi(s, k, \{k_i\}) \equiv \begin{cases} 1 & \text{if } \sum_i k_i = k, k_s = 1, \text{ and } s = 1, \dots, n, \\ 1 & \text{if } \sum_i k_i = k, k_{\hat{s}} = 0, \text{ and } s = n + 1, \dots, 2n - 1, \\ 0 & \text{otherwise.} \end{cases} \quad (\text{S24})$$

Since the eigenvalues of  $\mathbf{P}$  are assumed to be distinct, we have  $\frac{1}{4} = \bar{\alpha}_2 < \dots < \bar{\alpha}_n$ . We have numerically verified that this condition holds for all networks considered in the main text. We first seek to show that the matrix  $\mathbf{G}$  is non-singular by proving that the  $s$ th and  $s'$ th columns of

$\mathbf{G}$  are linearly independent for all distinct pairs  $s$  and  $s'$ . To do this, we first note that Eq. (S23) simplifies in the special cases  $k = 1$ ,  $k = 2$ ,  $k = 2n - 2$ , and  $k = 2n - 1$ , as follows.

For  $k = 1$ , to satisfy  $\sum_i k_i = k$ , we must have  $k_i = 1$  for exactly one value of  $i$  and  $k_i = 0$  for all the others (recall that each  $k_i$  is either 0, 1, or 2). For the case  $1 \leq s \leq n$ , we can derive a simplified formula, but it is not needed below, so we will skip that case here. For the case  $n + 1 \leq s \leq 2n - 1$ , to have  $\chi(s, k, \{k_i\}) = 1$  in Eq. (S24) we must have  $k_t = 1$  for some  $t \neq \hat{s}$  and  $k_i = 0$  for all  $i \neq t$  (including  $i = \hat{s}$ ). Since there are  $n - 1$  possibilities for  $t$ , there are that many nonzero terms in the summation in Eq. (S23), which reduces to

$$G_{1s} = \sum_{t \neq \hat{s}} \prod_{i \neq \hat{s}} a_i^{(k_i)} = \sum_{t \neq \hat{s}} \prod_{i \neq t, \hat{s}} \bar{\alpha}_i, \quad n + 1 \leq s \leq 2n - 1. \quad (\text{S25})$$

For  $k = 2$ , the condition  $\sum_i k_i = k$  implies that we either have (a)  $k_i = 2$  for exactly one value of  $i$  and  $k_i = 0$  for all the others, or (b)  $k_i = 1$  for two different values of  $i$ , and  $k_i = 0$  for all the others. For  $1 \leq s \leq n$ , we have  $\chi(s, k, \{k_i\}) = 0$  for the terms in Eq. (S23) corresponding to case (a), according to Eq. (S24). For nonzero terms in Eq. (S23) corresponding to case (b), we have  $k_s = 1$ ,  $k_t = 1$  with some  $t \neq s$ , and  $k_i = 0$  for all  $i \neq s, t$ . Putting the two cases together, we obtain

$$G_{2s} = \sum_{t \neq s} \prod_{i \neq s} a_i^{(k_i)} = \sum_{t \neq s} \prod_{i \neq t, s} \bar{\alpha}_i, \quad 1 \leq s \leq n. \quad (\text{S26})$$

A simplified expression for  $G_{2s}$  for  $n + 1 \leq s \leq 2n - 1$  can also be obtained, but it is not needed for our purpose.

For  $k = 2n - 2$ , satisfying  $\sum_i k_i = k$  requires that either (a)  $k_i = 0$  for exactly one value of  $i$  and  $k_i = 2$  for all the others, or (b)  $k_i = 1$  for two different values of  $i$ , and  $k_i = 2$  for all the others. For  $1 \leq s \leq n$ , similarly to the case of  $k = 2$ , there is no nonzero term in Eq. (S23) corresponding to case (a), and for the nonzero terms in Eq. (S23) corresponding to case (b), we have  $k_s = 1$ ,  $k_t = 1$  with some  $t \neq s$ , and  $k_i = 2$  for all  $i \neq s, t$ . Putting these two cases together, we obtain

$$G_{2n-2,s} = \sum_{t \neq s} \prod_{i \neq s} a_i^{(k_i)} = \sum_{t \neq s} 1 = n - 1, \quad 1 \leq s \leq n. \quad (\text{S27})$$

For  $n + 1 \leq s \leq 2n - 1$ , case (b) does not correspond to any nonzero term in Eq. (S23) because  $k_i \neq 0$  for all  $i$ . Case (a), on the other hand, yields exactly one term with  $k_{\hat{s}} = 0$ , leading to

$$G_{2n-2,s} = \prod_{i \neq \hat{s}} a_i^{(k_i)} = 1, \quad n + 1 \leq s \leq 2n - 1. \quad (\text{S28})$$

For  $k = 2n - 1$ , the only way to satisfy  $\sum_i k_i = k$  is to have just one  $k_i = 1$  and all the other  $k_i = 2$ . For  $1 \leq s \leq n$ , we must have  $k_s = 1$  for a nonzero term, so only one term survives in Eq. (S23), and hence

$$G_{2n-1,s} = \prod_{i \neq s} a_i^{(k_i)} = 1, \quad 1 \leq s \leq n. \quad (\text{S29})$$